theories/weakestpre/wp_tactics.v
@@ -52,10 +52,10 @@ Ltac wp_step' :=
       tac_change_goal (wp_par_ret_left _ _ _ _ _ _ _)
   | |- environments.envs_entails _ (wp _ _ (try (ret _) _ _) _) =>
       tac_change_goal (wp_try_ret _ _ _ _ _ _)
-  | |- environments.envs_entails _ (wp _ _ (stop Eval _) _) =>
+  | |- environments.envs_entails _ (wp _ _ (stop CEval _) _) =>
       first [ tac_change_goal (wp_eval_ret _ _ _ _ _)
             | tac_change_goal (wp_eval _ _ _ _ _ _) ]
-  | |- environments.envs_entails _ (wp _ _ (Stop Flip _ _) _) =>
+  | |- environments.envs_entails _ (wp _ _ (Stop CFlip _ _) _) =>
       tac_change_goal (wp_flip _ _ _ _ _)
   end.
 
