tutorial/tutorial.v
@@ -211,7 +211,7 @@ Goal ∀ η e body,
     b ← as_bool (eval η e) ;
     if (b : bool) then
       _ ← eval η body ;
-      stop Eval (η, EWhile e body)
+      stop CEval (η, EWhile e body)
     else
       ok. (* .no-goals *)
 Proof. (* .none *)
@@ -335,7 +335,7 @@ following five forms:
 * `Ret a` represents a computation that is finished
   and has produced a result `a`.
 
-* `Fail` represents a computation that has encountered a serious problem
+* `Crash` represents a computation that has encountered a serious problem
   and crashed. This is a situation that we want to avoid, and this is the
   purpose of the program logic that we wish to set up.
 
@@ -395,7 +395,7 @@ of computations*, equipped with the facilities that are needed to write
 the interpreter in a natural style. On the other hand, from a concrete
 point of view, it offers *a syntactic representation of a collection of
 threads*. The constructor `Par`  allows describing a binary tree of
-threads. At the leaves, the constructors `Ret`, `Fail`, and `Next`
+threads. At the leaves, the constructors `Ret`, `Crash`, and `Next`
 represent threads that have finished (in one way or another), while
 the constructor `Stop` represents a thread that is paused and needs
 to continue.
@@ -430,7 +430,7 @@ uses the following set of codes:
 Print code. (* .unfold *)
 
 (*|
-The code `Eval`, which we have encountered earlier, is used to request
+The code `CEval`, which we have encountered earlier, is used to request
 a recursive invocation of the function `eval`. The code `Loop` plays a
 similar role, but is used in the interpretation of `for` loops. The
 code `Flip` is used to request a Boolean value from the system: it is
@@ -482,7 +482,7 @@ Print step. (* .fold *)
 
 (*|
 Let us look at some of the cases in this definition.
-An `Eval` request steps to an invocation of `eval`:
+An `CEval` request steps to an invocation of `eval`:
 |*)
 
 Check @StepEval. (* .unfold *)
@@ -533,10 +533,10 @@ Safety
 (*|
 This reduction semantics allows us to define what it means for a program
 to be safe. A program is *safe* if it cannot crash, that is, if it cannot
-reduce (in zero, one, or more steps) to `Fail`.
+reduce (in zero, one, or more steps) to `Crash`.
 
 Technically, we say that a program is *initially safe* for `n` steps
-if it cannot reduce in at most `n` steps to `Fail`.
+if it cannot reduce in at most `n` steps to `Crash`.
 We say that a program is safe
 if, for every `n`, this program is initially safe for `n` steps.
 |*)
